lean/rewrite.lean
@@ -1,0 +1,75 @@
+lemma L1 : ∀ (f : ℕ → ℕ) (k : ℕ), f 0 = 0 → k = 0 → f k = 0 :=
+  assume f k H1 H2,
+    begin
+      rw H2,
+      rw H1
+    end
+
+#check L1
+
+lemma L2 : ∀ (x y : ℕ) (p : nat → Prop) (q : Prop), (q → x = y) → p y → q → p x :=
+  assume x y p q H1 H2 H3,
+    begin
+      rw H1; assumption
+    end
+
+#check L2
+
+
+lemma L3 : ∀ (f : ℕ → ℕ) (a b : ℕ), a = b → f a = 0 → f b = 0 :=
+  assume f a b H1 H2,
+    begin
+      rw [←H1, H2]
+    end
+
+lemma L4 : ∀ (a b c : ℕ), a + b + c = a + c + b :=
+  assume a b c, by rw [add_assoc, add_comm b, ←add_assoc]
+
+#check L4
+
+
+lemma L5 : ∀ (a b c : ℕ), a + b + c = a + c + b :=
+  assume a b c,
+    begin
+      rw [add_assoc, add_assoc, add_comm b]
+    end
+
+#check L5
+
+lemma L6 : ∀ (a b c : ℕ), a + b + c = a + c + b :=
+  assume a b c,
+    begin
+      rw [add_assoc, add_assoc, add_comm _ b]
+    end
+
+#check L6
+
+
+lemma L7 : ∀ (f : ℕ → ℕ) (a : ℕ), a + 0 = 0 → f a = f 0 :=
+  assume f a H,
+    begin
+      rw add_zero at H,
+      rw H
+    end
+
+-- rewrite can be used for Set, not just Prop
+
+universe u
+
+def tuple (α : Type u) (n : ℕ) := { l : list α // list.length l = n}
+
+#print tuple
+
+
+def ex1 {α : Type u} (n : ℕ) (H:n = 0) (t:tuple α n) : tuple α 0 :=
+  begin
+    rw H at t, assumption
+  end
+
+#check @ex1
+
+def ex2 {α : Type u} [ring α] (a b c : α) :
+  a * 0 + 0 * b + c * 0 + 0 * a = 0 :=
+    begin
+    end
+  _
