agda/plfa/relations.agda
@@ -1,0 +1,38 @@
+import Relation.Binary.PropositionalEquality as Eq
+open Eq using (_≡_; refl; cong)
+open import Data.Nat using (ℕ; zero; suc; _+_)
+open import Data.Nat.Properties using (+-comm)
+
+data _≤_ : ℕ → ℕ → Set where
+  z≤n : ∀ {n : ℕ}
+      -----------
+    → zero ≤ n
+
+  s≤s : ∀ {m n : ℕ}
+    → m ≤ n
+      -------------
+    → suc m ≤ suc n
+
+
+_ : 2 ≤ 4
+_ = s≤s (s≤s z≤n)
+
+infix 4 _≤_             -- binds less tightly than _+_
+
+_ : 1 + 2 ≤ 3           -- no paranthesis needed
+_ = s≤s (s≤s (s≤s z≤n)) -- way more verbose than coq's le_n
+
+inv-s≤s : ∀ {m n : ℕ}
+  → suc m ≤ suc n
+    -------------
+  → m ≤ n
+
+inv-s≤s (s≤s m≤n) = m≤n
+
+
+inv-z≤n : ∀ {n : ℕ}
+  → n ≤ zero
+    --------
+  → n ≡ zero
+
+inv-z≤n z≤n = refl
