agda/plfa/std.agda
@@ -1,0 +1,3 @@
+import Data.Nat.Properties using (+-assoc;+-suc;+-comm)
+
+-- +-identity... cannot type superscript r with \^r, is this due to lean ?
